more towards gnf_of

Replace_Terminals.thy
@@ -1,5 +1,5 @@
 theory Replace_Terminals
-  imports Context_Free_Grammar.Context_Free_Grammar
+  imports Greibach_Normal_Form.Greibach_Normal_Form
 begin
 
 (* unused, but a better replacement for inj_on_cong *)
@@ -29,7 +29,10 @@ lemma fresh_map_notIn: "finite A \<Longrightarrow> x \<in> set xs \<Longrightarr
   apply (induction xs arbitrary: A)
   by (auto simp: Let_def fresh0_notIn)
 
-lemma inj_on_fresh_map: "finite A \<Longrightarrow> inj_on (fresh_map A xs) (set xs)"
+lemma fresh_map_disj: "finite A \<Longrightarrow> B \<subseteq> A \<Longrightarrow> X \<subseteq> set xs \<Longrightarrow> B \<inter> fresh_map A xs ` X = {}"
+  by (force simp: fresh_map_notIn)
+
+lemma fresh_map_inj_on: "finite A \<Longrightarrow> inj_on (fresh_map A xs) (set xs)"
 proof (induction xs arbitrary: A)
   case Nil
   show ?case by simp
@@ -50,53 +53,54 @@ qed
 lemma fresh_map_distinct:
   assumes fin: "finite A"
   shows "distinct (map (fresh_map A xs) xs) \<longleftrightarrow> distinct xs" (is "?l \<longleftrightarrow> ?r")
-  using inj_on_fresh_map[OF fin] by (auto simp: distinct_map)
+  using fresh_map_inj_on[OF fin] by (auto simp: distinct_map)
 
-definition Replace_grammar where
-"Replace_grammar f as = (\<lambda>a. (f a, [Tm a])) ` as"
+definition Replace_Tm_new where
+"Replace_Tm_new f as = (\<lambda>a. (f a, [Tm a])) ` as"
 
-definition replace_grammar where
-"replace_grammar f as = [(f a, [Tm a]). a \<leftarrow> as]"
+definition replace_Tm_new where
+"replace_Tm_new f as = [(f a, [Tm a]). a \<leftarrow> as]"
 
-lemma set_replace_grammar: "set (replace_grammar f as) = Replace_grammar f (set as)"
-  by (auto simp: replace_grammar_def Replace_grammar_def)
+lemma set_replace_Tm_new: "set (replace_Tm_new f as) = Replace_Tm_new f (set as)"
+  by (auto simp: replace_Tm_new_def Replace_Tm_new_def)
 
-lemma Lhss_Replace_grammar: "Lhss (Replace_grammar f as) = f ` as"
-  by (simp add: Replace_grammar_def Lhss_image_Pair)
+lemma Lhss_Replace_Tm_new: "Lhss (Replace_Tm_new f as) = f ` as"
+  by (simp add: Replace_Tm_new_def Lhss_image_Pair)
 
-lemma Rhss_Replace_grammar:
+lemma Rhss_Replace_Tm_new:
   assumes inj: "inj_on f as" and a: "a \<in> as"
-  shows "Rhss (Replace_grammar f as) (f a) = {[Tm a]}"
-  by (auto simp: Replace_grammar_def Rhss_image_Pair_inj_on[OF inj a])
+  shows "Rhss (Replace_Tm_new f as) (f a) = {[Tm a]}"
+  by (auto simp: Replace_Tm_new_def Rhss_image_Pair_inj_on[OF inj a])
 
-lemma Rhss_Un_Replace_grammar:
+lemma Rhss_Un_Replace_Tm_new:
   assumes inj: "inj_on f as" and a: "a \<in> as" and fa: "f a \<notin> Lhss P"
-  shows "Rhss (P \<union> Replace_grammar f as) (f a) = {[Tm a]}"
-  by (simp add: Rhss_Un Rhss_Replace_grammar[OF inj a] fa[unfolded notin_Lhss_iff_Rhss])
+  shows "Rhss (P \<union> Replace_Tm_new f as) (f a) = {[Tm a]}"
+  by (simp add: Rhss_Un Rhss_Replace_Tm_new[OF inj a] fa[unfolded notin_Lhss_iff_Rhss])
 
-lemma Lang_Replace_grammar1:
+lemma Lang_Replace_Tm_new1:
   assumes inj: "inj_on f as" and a: "a \<in> as"
     and faP: "f a \<notin> Lhss P" and A: "A \<noteq> f a"
-  shows "Lang (insert (A, \<alpha> @ Nt (f a) # \<beta>) (P \<union> Replace_grammar f as)) =
-         Lang (insert (A, \<alpha> @ Tm a # \<beta>) (P \<union> Replace_grammar f as))"
+  shows "Lang (insert (A, \<alpha> @ Nt (f a) # \<beta>) (P \<union> Replace_Tm_new f as)) =
+         Lang (insert (A, \<alpha> @ Tm a # \<beta>) (P \<union> Replace_Tm_new f as))"
 proof-
-  note Rhss = Rhss_Un_Replace_grammar[OF inj a faP]
+  note Rhss = Rhss_Un_Replace_Tm_new[OF inj a faP]
   note * = Lang_subst1[OF A Rhss, where \<alpha> = \<alpha> and \<gamma> = \<beta>, simplified]
   show ?thesis by (simp add: *)
 qed
 
-definition replace_sym where
-"replace_sym f x = (case x of Tm a \<Rightarrow> Nt (f a) | _ \<Rightarrow> x)"
+definition replace_Tm_sym where
+"replace_Tm_sym f x = (case x of Tm a \<Rightarrow> Nt (f a) | _ \<Rightarrow> x)"
 
-lemma replace_sym_Nt: "replace_sym f (Nt A) = Nt A"
-  and replace_sym_Tm: "replace_sym f (Tm a) = Nt (f a)"
-  by (auto simp: replace_sym_def)
+lemma replace_Tm_sym_simps[simp]:
+  "replace_Tm_sym f (Nt A) = Nt A"
+  "replace_Tm_sym f (Tm a) = Nt (f a)"
+  by (auto simp: replace_Tm_sym_def)
 
-lemma Lang_Replace_grammar_append:
+lemma Lang_replace_Tm_sym:
   assumes inj: "inj_on f as" and Pfas: "Lhss P \<inter> f ` as = {}" and Afas: "A \<notin> f ` as"
-  defines "P' \<equiv> P \<union> Replace_grammar f as"
+  defines "P' \<equiv> P \<union> Replace_Tm_new f as"
   shows "Tms_syms \<beta> \<subseteq> as \<Longrightarrow>
- Lang (insert (A, \<alpha> @ map (replace_sym f) \<beta>) P') = Lang (insert (A, \<alpha> @ \<beta>) P')"
+ Lang (insert (A, \<alpha> @ map (replace_Tm_sym f) \<beta>) P') = Lang (insert (A, \<alpha> @ \<beta>) P')"
 proof (induction \<beta> arbitrary: \<alpha>)
   case Nil
   show ?case by simp
@@ -107,53 +111,37 @@ next
   show ?case
   proof (cases x)
     case (Nt A)
-    with IH show ?thesis by (auto simp: replace_sym_Nt)
+    with IH show ?thesis by simp
   next
     case [simp]: (Tm a)
     from Cons.prems have a: "a \<in> as" by auto
     from a Pfas have fa: "f a \<notin> Lhss P" by auto
     from a Afas have A: "A \<noteq> f a" by auto
-    note * = Lang_Replace_grammar1[OF inj a fa A]
-    from IH show ?thesis by (simp add: replace_sym_Tm * P'_def)
+    note * = Lang_Replace_Tm_new1[OF inj a fa A]
+    from IH show ?thesis by (simp add: * P'_def)
   qed
 qed
 
-definition map_tl where
-"map_tl f xs = (case xs of x#xs' \<Rightarrow> x # map f xs' | _ \<Rightarrow> xs)"
+definition replace_Tm_tl_syms where
+"replace_Tm_tl_syms f xs = (case xs of x#xs' \<Rightarrow> x # map (replace_Tm_sym f) xs' | _ \<Rightarrow> xs)"
 
-lemma map_tl_simps[simp]:
-"map_tl f [] = []"
-"map_tl f (x#xs) = x # map f xs"
-  by (auto simp: map_tl_def)
+definition replace_Tm_tl where
+"replace_Tm_tl f P = [(A, replace_Tm_tl_syms f \<alpha>). (A,\<alpha>) \<leftarrow> P] @ replace_Tm_new f (tms P)"
 
-lemma Lang_map_tl_replace:
+lemma Lang_replace_Tm_tl_syms:
   assumes pre: "inj_on f as" "Lhss P \<inter> f ` as = {}" "A \<notin> f ` as"
     and \<alpha>: "Tms_syms \<alpha> \<subseteq> as"
-  defines "P' \<equiv> P \<union> Replace_grammar f as"
-  shows "Lang (insert (A, map_tl (replace_sym f) \<alpha>) P') = Lang (insert (A,\<alpha>) P')"
+  defines "P' \<equiv> P \<union> Replace_Tm_new f as"
+  shows "Lang (insert (A, replace_Tm_tl_syms f \<alpha>) P') = Lang (insert (A,\<alpha>) P')"
 proof (cases \<alpha>)
   case Nil
-  then show ?thesis by simp
+  then show ?thesis by (simp add: replace_Tm_tl_syms_def)
 next
   case [simp]: (Cons x \<beta>)
   with \<alpha> have \<beta>: "Tms_syms \<beta> \<subseteq> as" by simp
-  from Lang_Replace_grammar_append[OF pre \<beta>, where \<alpha> = "[x]"]
-  show ?thesis by (simp add: P'_def)
+  from Lang_replace_Tm_sym[OF pre \<beta>, where \<alpha> = "[x]"]
+  show ?thesis by (simp add: replace_Tm_tl_syms_def P'_def)
 qed
-
-definition replace_tl where
-"replace_tl f P = [(A, map_tl (replace_sym f) \<alpha>). (A,\<alpha>) \<leftarrow> P]"
-
-lemma "replace_tl f = map (map_prod id (map_tl (replace_sym f)))"
-  by (simp add: fun_eq_iff replace_tl_def split: prod.split)
-
-lemma replace_tl_simps[simp]:
-"replace_tl f [] = []"
-"replace_tl f ((A,\<alpha>)#P) = (A, map_tl (replace_sym f) \<alpha>) # replace_tl f P"
-  by (simp_all add: replace_tl_def)
-
-definition replace_Tm_tl where
-"replace_Tm_tl f P = replace_tl f P @ replace_grammar f (tms P)"
 
 lemma lang_replace_Tm_tl:
   assumes inj: "inj_on f (Tms (set P))" and Nts: "Nts (set P) \<inter> f ` Tms (set P) = {}"
@@ -166,7 +154,8 @@ proof-
       and Pfas: "Lhss (set P) \<inter> f ` as = {}"
       and Pas: "Tms (set P) \<subseteq> as"
     from Pfas Pas
-    have "\<And>Q. Lhss Q \<inter> f ` as = {} \<Longrightarrow> Lang (Q \<union> set (replace_tl f P) \<union> Replace_grammar f as) = Lang (Q \<union> set P \<union> Replace_grammar f as)"
+    have "\<And>Q. Lhss Q \<inter> f ` as = {} \<Longrightarrow> Lang (Q \<union> set [(A, replace_Tm_tl_syms f \<alpha>). (A,\<alpha>) \<leftarrow> P] \<union> Replace_Tm_new f as) = Lang (Q \<union> set P \<union> Replace_Tm_new f as)"
+      apply simp
     proof (induction P)
       case Nil
       show ?case by simp
@@ -183,21 +172,94 @@ proof-
         from Afas Qfas have "Lhss (Q \<union> {(A,\<alpha>')}) \<inter> f ` as = {}" for \<alpha>' by (simp add: ac_simps)
         note IH = Cons.IH[OF this Pfas Pas, simplified]
         from Pfas Qfas have QPfas: "Lhss (Q \<union> set P) \<inter> f ` as = {}" by auto
-        from Lang_map_tl_replace[OF inj QPfas Afas \<alpha>as]
-        show ?thesis by (simp add: IH)
+        note * = Lang_replace_Tm_tl_syms[OF inj QPfas Afas \<alpha>as]
+        show ?thesis by (simp add: * IH)
       qed
     qed
   }
   from this[of "set (tms P)" "{}",simplified] inj Lhss
-  have 1: "lang (replace_Tm_tl f P) = Lang (set P \<union> Replace_grammar f (Tms (set P)))"
-    by (simp add: replace_Tm_tl_def set_tms set_replace_grammar)
+  have 1: "lang (replace_Tm_tl f P) = Lang (set P \<union> Replace_Tm_new f (Tms (set P)))"
+    by (simp add: replace_Tm_tl_def set_tms set_replace_Tm_new)
   have 2: "\<dots> A = lang P A"
     apply (subst Lang_Un_disj_Lhss[OF _ A])
-     apply (simp add: Lhss_Replace_grammar Nts) (* !? *)
+     apply (simp add: Lhss_Replace_Tm_new Nts) (* !? *)
     apply (rule refl).
   show ?thesis by (simp add: 1 2)
 qed
 
+definition replace_Tm_tl_fresh where
+"replace_Tm_tl_fresh P = replace_Tm_tl (fresh_map (Nts (set P)) (tms P)) P"
+
+lemma lang_replace_Tm_tl_fresh:
+  assumes A: "A \<in> Nts (set P)"
+  shows "lang (replace_Tm_tl_fresh P) A = lang P A"
+proof-
+  have fin: "finite (Nts (set P))" by (auto intro!: finite_Nts)
+  from fresh_map_inj_on[OF fin, where xs = "tms P"]
+    fresh_map_notIn[OF fin, where xs="tms P"]
+  show ?thesis
+    by (auto simp: replace_Tm_tl_fresh_def set_tms intro!: lang_replace_Tm_tl[OF _ _ A])
+qed
+
+definition GNF where
+"GNF P = (\<forall>(A,\<alpha>) \<in> P. \<exists>a Bs. \<alpha> = Tm a # map Nt Bs)"
+
+abbreviation gnf where
+"gnf P \<equiv> GNF (set P)"
+
+lemma GNF_I: "(\<And>A \<alpha>. (A,\<alpha>) \<in> P \<Longrightarrow> \<exists>a Bs. \<alpha> = Tm a # map Nt Bs) \<Longrightarrow> GNF P"
+  by (auto simp: GNF_def)
+
+lemma GNF_Un: "GNF (P \<union> Q) \<longleftrightarrow> GNF P \<and> GNF Q"
+  by (auto simp: GNF_def ball_Un)
+
+lemma gnf_replace_Tm_new: "gnf (replace_Tm_new f as)"
+  by (auto intro!: GNF_I simp: replace_Tm_new_def)
+
+lemma gnf_replace_Tm_tl:
+  assumes P: "gnf_hd P"
+  shows "gnf (replace_Tm_tl f P)"
+  apply (unfold replace_Tm_tl_fresh_def replace_Tm_tl_def set_append GNF_Un)
+proof (intro conjI gnf_replace_Tm_new GNF_I)
+  fix A \<alpha>' assume "(A,\<alpha>') \<in> set [(A, replace_Tm_tl_syms f \<alpha>). (A,\<alpha>) \<leftarrow> P]"
+  then obtain \<alpha> where "(A,\<alpha>) \<in> set P" and \<alpha>': "\<alpha>' = replace_Tm_tl_syms f \<alpha>" by auto
+  with P obtain a \<beta> where "\<alpha> = Tm a # \<beta>" by (auto simp: GNF_hd_def)
+  with \<alpha>' have \<alpha>': "\<alpha>' = Tm a # map (replace_Tm_sym f) \<beta>" by (auto simp: replace_Tm_tl_syms_def)
+  define Bs where "Bs \<equiv> [case x of Nt B \<Rightarrow> B | Tm b \<Rightarrow> f b. x \<leftarrow> \<beta>]"
+  have "map (replace_Tm_sym f) \<beta> = map Nt Bs"
+    by (unfold Bs_def, induction \<beta>, auto split: sym.splits)
+  with \<alpha>' have "\<alpha>' = Tm a # map Nt Bs" by simp
+  then show "\<exists>a Bs. \<alpha>' = Tm a # map Nt Bs" by blast
+qed
+
+definition gnf_of where
+"gnf_of P = replace_Tm_tl (fresh_map (Nts (set P)) (tms P)) (gnf_hd_of P)"
+
+theorem gnf_gnf_of: "gnf (gnf_of P)"
+  apply (unfold gnf_of_def)
+  apply (rule gnf_replace_Tm_tl)
+  using gnf_hd_gnf_hd_of.
+
+lemma Tms_GNF_hd_of: "Tms (GNF_hd_of As P) \<subseteq> Tms P" sorry
+
+theorem lang_gnf_of:
+  assumes A: "A \<in> set (nts P)"
+  shows "lang (gnf_of P) A = lang P A - {[]}"
+  apply (fold lang_gnf_hd_of[OF A])
+  apply (unfold gnf_of_def)
+proof (rule lang_replace_Tm_tl)
+  define f where "f = fresh_map (Nts (set P)) (tms P)"
+  show "inj_on f (Tms (set (gnf_hd_of P)))"
+    apply (unfold f_def)
+    apply (rule inj_on_subset[OF fresh_map_inj_on])
+    by (simp_all add: finite_Nts set_tms set_gnf_hd_of Tms_GNF_hd_of)
+  show "Nts (set (gnf_hd_of P)) \<inter>
+    f ` Tms (set (gnf_hd_of P)) = {}"
+    apply (unfold f_def)
+    apply (fold set_tms)
+    apply (rule fresh_map_disj)
+    apply (auto simp: finite_Nts set_gnf_hd_of)
+    oops
 
 
 end
